src/SepCancel.v
@@ -3,7 +3,7 @@ Require Import SepTheoryX PropX.
 Require Import PropXTac.
 Require Import RelationClasses EqdepClass.
 Require Import Expr ExprUnify2.
-Require Import DepList.
+Require Import SepExpr SepHeap.
 Require Import Setoid.
 Require Import Prover.
 Require Import SepExpr.
@@ -11,22 +11,17 @@ Require Import SepExpr.
 Set Implicit Arguments.
 Set Strict Implicit.
 
-Require NatMap Multimap.
-
-Module FM := NatMap.IntMap.
-Module MM := Multimap.Make FM.
-Module MF := NatMap.MoreFMapFacts FM.
-
-Definition BadInj types (e : expr types) := False.
-Definition BadPred (f : func) := False.
-Definition BadPredApply types (f : func) (es : list (expr types)) (_ : env types) := False.
-
-Module SepCancler (SE : SepExprType).
+Module Make (U : SynUnifier) (SH : SepHeap).
+  Module Import SE := SH.SE.
+  Module Import SEP_FACTS := SepExprFacts SE.
 
   Section env.
     Variable types : list type.
     Variable pcType : tvar.
     Variable stateType : tvar.
+
+    Variable funcs : functions types.
+    Variable preds : SE.predicates types pcType stateType.
 
     (** The actual tactic code **)
     Variable Prover : ProverT types.
@@ -49,18 +44,19 @@ Module SepCancler (SE : SepExprType).
         end.
     End fold_left3_opt.
 
-    Definition unifyArgs (bound : nat) (summ : Facts Prover) (l r : list (expr types)) (ts : list tvar) (sub : Subst types)
-      : option (Subst types) :=
+
+    Definition unifyArgs (bound : nat) (summ : Facts Prover) (l r : list (expr types)) (ts : list tvar) (sub : U.Subst types)
+      : option (U.Subst types) :=
       fold_left_3_opt 
-        (fun l r t (acc : Subst _) =>
+        (fun l r t (acc : U.Subst _) =>
           if Prove Prover summ (Expr.Equal t l r)
             then Some acc
-            else exprUnify bound l r acc)
+            else U.exprUnify bound l r acc)
         l r ts sub.
 
     Fixpoint unify_remove (bound : nat) (summ : Facts Prover) (l : exprs types) (ts : list tvar) (r : list (exprs types))
-      (sub : Subst types)
-      : option (list (list (expr types)) * Subst types) :=
+      (sub : U.Subst types)
+      : option (list (list (expr types)) * U.Subst types) :=
         match r with 
           | nil => None
           | a :: b => 
@@ -73,22 +69,6 @@ Module SepCancler (SE : SepExprType).
               | Some sub => Some (b, sub)
             end
         end.
-(*
-    Fixpoint unify_remove_all (bound : nat) (summ : Facts Prover) (l r : list (list (expr types))) (ts : list tvar)
-      (sub : Subst types)
-      : list (list (expr types)) * list (list (expr types)) * Subst types :=
-        match l with
-          | nil => (l, r, sub)
-          | a :: b => 
-            match unify_remove bound summ a ts r sub with
-              | None => 
-                let '(l,r,sub) := unify_remove_all bound summ b r ts sub in
-                (a :: l, r, sub)
-              | Some (r, sub) =>
-                unify_remove_all bound summ b r ts sub
-            end
-        end.
-*)
 
     Require Ordering.
 
@@ -126,29 +106,31 @@ Module SepCancler (SE : SepExprType).
         Ordering.insert_in_order _ meta_order_funcs (args, k) acc)) imps nil.
 
     Lemma impuresD'_flatten : forall U G cs imps,
-      heq U G cs (impuresD' imps)
-                 (starred' (fun v => Func (snd v) (fst v)) 
-                           (FM.fold (fun f argss acc => 
-                             map (fun args => (args, f)) argss ++ acc) imps nil) Emp).
+      SE.heq funcs preds U G cs
+        (SH.impuresD _ _ imps)
+        (SH.starred (fun v => SE.Func (snd v) (fst v)) 
+          (FM.fold (fun f argss acc => 
+            map (fun args => (args, f)) argss ++ acc) imps nil) SE.Emp).
     Proof.
-      unfold impuresD'. clear. intros. generalize Emp at 2 3.
-      eapply MM.PROPS.fold_rec; intros.
-        eapply MM.PROPS.fold_Empty; eauto with typeclass_instances.
+      clear. intros. eapply MM.PROPS.fold_rec; intros.
+        rewrite (SH.impuresD_Empty funcs preds U G cs H).
+        rewrite SH.starred_def. simpl. reflexivity.
 
-        rewrite MM.PROPS.fold_Add; eauto with typeclass_instances hprop.
-        rewrite starred'_app. symmetry. rewrite <- starred'_base.
-        rewrite H2.
-        eapply heq_star_frame; try reflexivity. clear.
-        induction e; simpl; intros; try reflexivity.
+        rewrite SH.impuresD_Add; eauto. rewrite SH.starred_app. 
+        rewrite H2. symmetry. rewrite SH.starred_base. heq_canceler.
+        repeat rewrite SH.starred_def.
+        clear; induction e; simpl; intros; try reflexivity.
         rewrite IHe. reflexivity.
     Qed.
 
-    Lemma starred'_perm : forall T L R,
+    Lemma starred_perm : forall T L R,
       Permutation.Permutation L R ->
       forall (F : T -> _) U G cs base,
-      heq U G cs (starred' F L base) (starred' F R base).
+      heq funcs preds U G cs (SH.starred F L base) (SH.starred F R base).
     Proof.
-      clear. induction 1; simpl; intros;
+      clear. intros.
+      repeat rewrite SH.starred_def.
+      induction H; simpl; intros;
       repeat match goal with
                | [ H : _ |- _ ] => rewrite H
              end; try reflexivity; heq_canceler.
@@ -179,24 +161,25 @@ Module SepCancler (SE : SepExprType).
     Qed.
 
     Lemma order_impures_D : forall U G cs imps,
-      heq U G cs (impuresD' imps)
-                 (starred' (fun v => (Func (snd v) (fst v))) (order_impures imps) Emp).
+      heq funcs preds U G cs 
+        (SH.impuresD _ _ imps)
+        (SH.starred (fun v => (Func (snd v) (fst v))) (order_impures imps) Emp).
     Proof.
       clear. intros. rewrite impuresD'_flatten. unfold order_impures.
-      eapply starred'_perm. eapply fold_Permutation. reflexivity.
+      eapply starred_perm. eapply fold_Permutation. reflexivity.
     Qed.
     
     (** NOTE : l and r are reversed here **)
     Fixpoint cancel_in_order (bound : nat) (summ : Facts Prover) 
-      (ls : cancel_list) (acc rem : MM.mmap (exprs types)) (sub : Subst types) 
-      : MM.mmap (exprs types) * MM.mmap (exprs types) * Subst types :=
+      (ls : cancel_list) (acc rem : MM.mmap (exprs types)) (sub : U.Subst types) 
+      : MM.mmap (exprs types) * MM.mmap (exprs types) * U.Subst types :=
       match ls with
         | nil => (acc, rem, sub)
         | (args,f) :: ls => 
           match MM.FM.find f rem with
             | None => cancel_in_order bound summ ls (MM.mmap_add f args acc) rem sub
             | Some argss =>
-              match nth_error sfuncs f with
+              match nth_error preds f with
                 | None => cancel_in_order bound summ ls (MM.mmap_add f args acc) rem sub (** Unused! **)
                 | Some ts => 
                   match unify_remove bound summ args (SDomain ts) argss sub with
@@ -210,60 +193,41 @@ Module SepCancler (SE : SepExprType).
 
     Lemma cancel_in_orderOk : forall U G cs bound summ ls acc rem sub L R S,
       cancel_in_order bound summ ls acc rem sub = (L, R, S) ->
-      himp U G cs (impuresD' R) (impuresD' L) ->
-      himp U G cs (impuresD' acc) (Star (starred' (fun v => (Func (snd v) (fst v))) ls Emp)
-                                        (impuresD' acc)).
+      himp funcs preds U G cs (SH.impuresD _ _ R) (SH.impuresD _ _ L) ->
+      himp funcs preds U G cs 
+        (SH.impuresD _ _ acc)
+        (Star (SH.starred (fun v => (Func (snd v) (fst v))) ls Emp)
+              (SH.impuresD _ _ acc)).
     Proof.
       
     Admitted.
 
 
-    Definition sepCancel (bound : nat) (summ : Facts Prover) (l r : SHeap) :
-      SHeap * SHeap * Subst types :=
-      let ordered_r := order_impures (impures r) in
-      let sorted_l := MM.FM.map (fun v => Ordering.sort _ meta_order_args v) (impures l) in 
+    Definition sepCancel (bound : nat) (summ : Facts Prover) (l r : SH.SHeap types pcType stateType) :
+      SH.SHeap _ _ _ * SH.SHeap _ _ _ * U.Subst types :=
+      let ordered_r := order_impures (SH.impures r) in
+      let sorted_l := MM.FM.map (fun v => Ordering.sort _ meta_order_args v) (SH.impures l) in 
       let '(rf, lf, sub) := 
-        cancel_in_order bound summ ordered_r (MM.empty _) sorted_l (empty_Subst _)
+        cancel_in_order bound summ ordered_r (MM.empty _) sorted_l (U.Subst_empty _)
       in
-      ({| impures := lf ; pures := pures l ; other := other l |},
-       {| impures := rf ; pures := pures r ; other := other r |},
+      ({| SH.impures := lf ; SH.pures := SH.pures l ; SH.other := SH.other l |},
+       {| SH.impures := rf ; SH.pures := SH.pures r ; SH.other := SH.other r |},
        sub).
 
-    Theorem sepCancel_correct : forall U G cs bound summ l r l' r' sub ,
+    Theorem sepCancel_correct : forall U G cs bound summ l r l' r' sub,
       Valid Prover_correct U G summ ->
       sepCancel bound summ l r = (l', r', sub) ->
-      himp U G cs (sheapD l) (sheapD r) ->
-      himp U G cs (sheapD l') (sheapD r').
+      himp funcs preds U G cs (SH.sheapD l) (SH.sheapD r) ->
+      U.Subst_equations funcs U G sub ->
+      himp funcs preds U G cs (SH.sheapD l') (SH.sheapD r').
     Proof.
       clear. destruct l; destruct r. unfold sepCancel. simpl.
       intros. repeat rewrite sheapD_sheapD'. repeat rewrite sheapD_sheapD' in H1.
-      destruct l'; destruct r'. unfold sheapD' in *. simpl in *.
+      destruct l'; destruct r'. 
 
       
     Admitted.
 
   End env.
-
-  Implicit Arguments Emp [ types pcType stateType ].
-  Implicit Arguments Star [ types pcType stateType ].
-  Implicit Arguments Exists [ types pcType stateType ].
-  Implicit Arguments Func [ types pcType stateType ].
-  Implicit Arguments Const [ types pcType stateType ].
-  Implicit Arguments Inj [ types pcType stateType ].
-
-
-  Lemma change_ST_himp_himp : forall (types : list type)
-    (funcs : functions types) (pc st : tvar)
-    (sfuncs : list (ssignature types pc st))
-    EG G
-    (cs : codeSpec (tvarD types pc) (tvarD types st))
-    (L R : sexpr types pc st),
-    himp funcs sfuncs EG G cs L R ->
-    ST.himp cs
-      (@sexprD types pc st funcs sfuncs EG G L)
-      (@sexprD types pc st funcs sfuncs EG G R).
-  Proof.
-    unfold himp. intros. auto.
-  Qed.
 
 End Make.
