src/SepHeap.v
@@ -1,0 +1,909 @@
+Require Import List.
+Require Import SepTheoryX PropX.
+Require Import PropXTac.
+Require Import RelationClasses EqdepClass.
+Require Import Expr SepExpr.
+Require Import DepList.
+Require Import Setoid.
+
+Set Implicit Arguments.
+Set Strict Implicit.
+
+Require NatMap Multimap.
+
+Module FM := NatMap.IntMap.
+Module MM := Multimap.Make FM.
+Module MF := NatMap.MoreFMapFacts FM.
+
+Module Type SepHeap.
+  Declare Module SE : SepExpr.
+
+  Section env.
+    Variable types : list type.
+    Variable pcType : tvar.
+    Variable stateType : tvar.
+
+    Record SHeap : Type :=
+    { impures : MM.mmap (exprs types)
+    ; pures   : list (expr types)
+    ; other   : list (SE.ST.hprop (tvarD types pcType) (tvarD types stateType) nil)
+    }.
+
+    (** TODO: What happens if I denote this directly to hprop?
+     ** - fewer lemmas about concrete syntax!
+     ** - can't re-hash (probably don't want to do this anyways...)
+     ** * I think this is Ok for now
+     **)
+    Parameter sheapD : SHeap -> SE.sexpr types pcType stateType.
+
+    (** Operations on [SHeap]s **)
+    Parameter star_SHeap : SHeap -> SHeap -> SHeap.
+
+    Parameter sheap_liftVars : nat -> nat -> SHeap -> SHeap.
+
+    Parameter sheapSubstU : nat -> nat -> nat -> SHeap -> SHeap.
+
+    (** Convert an [sexpr] to an [SHeap] **)
+    Parameter hash : SE.sexpr types pcType stateType -> variables * SHeap.
+
+    Parameter impuresD : MM.mmap (exprs types) -> SE.sexpr types pcType stateType.
+
+    Parameter starred : forall (T : Type) (F : T -> SE.sexpr types pcType stateType), 
+      list T -> SE.sexpr types pcType stateType -> SE.sexpr types pcType stateType.
+    
+    Section facts.
+      Variable funcs : functions types.
+      Variable preds : SE.predicates types pcType stateType.
+      Variables U G : env types.
+      Variable cs : codeSpec (tvarD types pcType) (tvarD types stateType).
+
+      (** Theorems **)
+      Axiom hash_denote : forall (s : SE.sexpr types pcType stateType), 
+        SE.heq funcs preds U G cs s (SE.existsEach (fst (hash s)) (sheapD (snd (hash s)))).
+
+      Axiom star_SHeap_denote : forall s s',
+        SE.heq funcs preds U G cs (SE.Star (sheapD s) (sheapD s')) (sheapD (star_SHeap s s')).
+
+      (** Definitions **)
+      Axiom starred_def : forall (T : Type) (F : T -> SE.sexpr _ _ _) (ls : list T) (base : SE.sexpr _ _ _),
+        SE.heq funcs preds U G cs 
+            (starred F ls base)
+            (fold_right (fun x a => SE.Star (F x) a) base ls).
+
+      Axiom starred_base : forall (T : Type) (F : T -> SE.sexpr _ _ _) (ls : list T) (base : SE.sexpr _ _ _),
+        SE.heq funcs preds U G cs 
+            (starred F ls base)
+            (SE.Star base (starred F ls SE.Emp)).
+
+      Axiom starred_app : forall (T : Type) (F : T -> SE.sexpr _ _ _) (ls ls' : list T) (base : SE.sexpr _ _ _),
+        SE.heq funcs preds U G cs 
+            (starred F (ls ++ ls') base)
+            (starred F ls (starred F ls' base)).
+
+      Axiom impuresD_Add : forall f argss i i',
+        MM.PROPS.Add f argss i i' ->
+        ~FM.In f i ->
+        SE.heq funcs preds U G cs
+            (impuresD i')
+            (SE.Star (starred (SE.Func f) argss SE.Emp) (impuresD i)).
+
+      Axiom impuresD_Empty : forall i,
+        FM.Empty i ->
+        SE.heq funcs preds U G cs
+            (impuresD i) SE.Emp.
+
+      Axiom sheapD_def : forall s,
+        SE.heq funcs preds U G cs
+            (sheapD s)
+            (SE.Star (impuresD (impures s))
+                     (SE.Star (starred (@SE.Inj _ _ _) (pures s) SE.Emp)
+                              (starred (@SE.Const _ _ _) (other s) SE.Emp))).
+    End facts.
+  End env.
+End SepHeap.
+
+Module Make (SE : SepExpr) <: SepHeap with Module SE := SE.
+  Module Import SE := SE.
+  Module ST := SE.ST.
+
+  Module Import SE_FACTS := SepExpr.SepExprFacts SE.
+
+  Section env.
+    Variable types : list type.
+    Variable pcType : tvar.
+    Variable stateType : tvar.
+
+    Variable funcs : functions types.
+    Variable preds : predicates types pcType stateType.
+
+    (** A more efficient representation for sexprs. **)
+    Record SHeap : Type :=
+    { impures : MM.mmap (exprs types)
+    ; pures   : list (expr types)
+    ; other   : list (ST.hprop (tvarD types pcType) (tvarD types stateType) nil)
+    }.
+  
+    Definition SHeap_empty : SHeap := 
+      {| impures := @MM.empty _
+       ; pures   := nil
+       ; other   := nil
+       |}.
+
+
+
+(*
+    Lemma fold_left_star : forall T a c cs F (ls : list T)  base,
+      heq funcs preds a c cs (fold_left (fun acc x => Star (F x) acc) ls base)
+      (Star (fold_left (fun acc x => Star (F x) acc) ls Emp) base).
+    Proof.
+      induction ls; simpl; intros.
+      rewrite heq_star_emp_l. reflexivity.
+      rewrite IHls. symmetry. rewrite IHls.
+      repeat rewrite heq_star_assoc. rewrite heq_star_emp_l. reflexivity.
+    Qed.
+
+    Ltac heq_fold_left_opener :=
+      match goal with
+        | [ |- context [ fold_left _ _ ?B ] ] =>
+          match B with
+            | Emp => fail 1 
+            | _ => rewrite fold_left_star with (base := B)
+          end
+      end.
+*)    
+
+    Existing Instance himp_rel_relation.
+    Existing Instance heq_rel_relation.
+    Hint Rewrite heq_star_emp_l heq_star_emp_r : hprop.
+
+    Theorem ST_himp_himp : forall (U G : env types) cs L R,
+      SE.himp funcs preds U G cs L R ->
+      ST.himp cs (sexprD funcs preds U G L) (sexprD funcs preds U G R).
+    Proof.
+      clear. auto.
+    Qed.
+
+    Theorem ST_heq_heq : forall (U G : env types) cs L R,
+      heq funcs preds U G cs L R ->
+      ST.heq cs (sexprD funcs preds U G L) (sexprD funcs preds U G R).
+    Proof.
+      clear. auto.
+    Qed.
+
+
+    (** lift all the "real" variables in [a,...) 
+     ** to the range [a+b,...)
+     **)
+    Fixpoint liftSExpr (a b : nat) (s : sexpr types pcType stateType) : sexpr _ _ _ :=
+      match s with
+        | Emp => Emp
+        | Inj p => Inj (liftExpr a b p)
+        | Star l r => Star (liftSExpr a b l) (liftSExpr a b r)
+        | Exists t s => 
+          Exists t (liftSExpr (S a) b s)
+        | Func f xs => Func f (map (liftExpr a b) xs)
+        | Const c => Const c
+      end.
+
+    (** lift all the "real" variables in [a,...) 
+     ** to the range [a+b,...)
+     **)
+    Definition liftSHeap (a b : nat) (s : SHeap) : SHeap :=
+      {| impures := MM.mmap_map (map (liftExpr a b)) (impures s)
+       ; pures   := map (liftExpr a b) (pures s)
+       ; other   := other s
+       |}.
+
+    Fixpoint star_SHeap (l r : SHeap) : SHeap :=
+      {| impures := MM.mmap_join (impures l) (impures r)
+       ; pures := pures l ++ pures r
+       ; other := other l ++ other r
+       |}.
+
+    Definition sheap_liftVars (from : nat) (delta : nat) (h : SHeap) : SHeap :=
+      {| impures := MM.mmap_map (map (liftExpr from delta)) (impures h)
+       ; pures := map (liftExpr from delta) (pures h)
+       ; other := other h
+       |}.
+
+    (** CURRENTLY NOT USED **)
+    Fixpoint substV types (vs : list nat) (e : expr types) : expr types :=
+      match e with
+        | Expr.Const _ c => Expr.Const c
+        | Var x => 
+          Var (match nth_error vs x with
+                 | None => x
+                 | Some y => y
+               end)
+        | UVar x => UVar x
+        | Expr.Func f xs => 
+          Expr.Func f (map (substV vs) xs)
+        | Equal t e1 e2 => Equal t (substV vs e1) (substV vs e2)
+        | Not e1 => Not (substV vs e1)
+      end.
+
+    Fixpoint hash (s : sexpr types pcType stateType) : ( variables * SHeap ) :=
+      match s with
+        | Emp => (nil, SHeap_empty)
+        | Inj p => (nil,
+          {| impures := MM.empty _
+           ; pures := p :: nil
+           ; other := nil
+           |})
+        | Star l r =>
+          let (vl, hl) := hash l in
+          let (vr, hr) := hash r in
+          let nr := length vr in
+          (vl ++ vr,
+            star_SHeap (sheap_liftVars 0 nr hl) (sheap_liftVars nr (length vl) hr))
+        | Exists t b =>
+          let (v, b) := hash b in
+          (t :: v, b)
+        | Func f a =>
+          (nil,
+           {| impures := MM.mmap_add f a (MM.empty _)
+            ; pures := nil
+            ; other := nil
+           |})
+        | Const c => 
+          (@nil tvar,
+           {| impures := MM.empty _
+            ; pures := @nil (expr types)
+            ; other := c :: nil
+            |})
+      end.
+
+    Definition starred (T : Type) (F : T -> sexpr types pcType stateType) (ls : list T) (base : sexpr _ _ _)
+      : sexpr _ _ _ :=
+      fold_right (fun x a => match a with 
+                               | Emp => F x
+                               | _ => Star (F x) a
+                             end) base ls.     
+
+    Definition sheapD (h : SHeap) : sexpr types pcType stateType :=
+      let a := starred (@Const _ _ _) (other h) Emp in
+      let a := starred (@Inj _ _ _) (pures h) a in
+      let a := MM.FM.fold (fun k => starred (Func k)) (impures h) a in
+      a.
+
+    Definition sheapD' (h : SHeap) : sexpr types pcType stateType :=
+      Star (MM.FM.fold (fun k => starred (Func k)) (impures h) Emp)
+           (Star (starred (@Inj _ _ _) (pures h) Emp)
+                 (starred (@Const _ _ _) (other h) Emp)).
+
+    Definition impuresD (imp : MM.mmap (exprs types)) : sexpr types pcType stateType :=
+      MM.FM.fold (fun k ls acc => 
+        Star (starred (Func k) ls Emp) acc) imp Emp.
+
+    Section with_envs.
+      Variables U G : env types.
+      Variable cs : codeSpec (tvarD types pcType) (tvarD types stateType).
+
+      Local Notation "a '<===>' b" := (heq funcs preds U G cs a b) (at level 60, only parsing).
+
+      Theorem starred_def : forall (T : Type) (F : T -> SE.sexpr _ _ _) (ls : list T) (base : SE.sexpr _ _ _),
+        (starred F ls base) <===>
+        (fold_right (fun x a => SE.Star (F x) a) base ls).
+      Proof.
+        induction ls; simpl; intros.
+          reflexivity.
+          specialize (IHls base). revert IHls.
+          case_eq (starred F ls base); intros;
+            rewrite <- IHls; heq_canceler.
+      Qed.
+
+      Theorem starred_base : forall T F ls base, 
+        (@starred T F ls base) <===> (SE.Star base (@starred T F ls Emp)).
+      Proof.
+        intros. repeat rewrite starred_def.
+        revert base. induction ls; simpl in *; intros.
+          heq_canceler.
+          rewrite IHls. heq_canceler.
+      Qed.
+      
+      Ltac heq_canceler :=
+        repeat match goal with
+                 | [ H : SE.heq _ _ _ _ _ _ _ |- _ ] => rewrite H
+                 | [ |- context [ starred ?F ?L ?B ] ] =>
+                   match B with
+                     | SE.Emp => fail 1
+                     | _ => rewrite (@starred_base _ F L B)
+                   end
+               end;
+        SE_FACTS.heq_canceler.
+
+      Global Add Parametric Morphism : (fun k0 : nat => starred (Func k0)) with
+        signature (eq ==> eq ==> heq funcs preds U G cs ==> heq funcs preds U G cs)
+        as star_himp_mor'.
+      Proof.
+        intros. repeat rewrite starred_def.
+        revert H. revert x; revert y1.
+        induction y0; unfold heq in *; simpl in *; intros; try eauto.
+        rewrite IHy0; eauto. heq_canceler.
+      Qed.
+
+      Lemma transpose_neqkey_starred : NatMap.IntMapProperties.transpose_neqkey (SE.heq funcs preds U G cs)
+        (fun k0 : nat => starred (Func k0)).
+      Proof.
+        red. intros. rewrite starred_base. symmetry.
+        rewrite starred_base. repeat rewrite starred_base with (base := a).
+        heq_canceler.
+      Qed.
+      Lemma transpose_neqkey_Star (X : Type) F : NatMap.IntMapProperties.transpose_neqkey (heq funcs preds U G cs)
+        (fun (k0 : nat) (ls : X) (a1 : sexpr types _ _) => Star (F k0 ls) a1).
+      Proof.
+        red. intros. heq_canceler.
+      Qed.
+
+      Hint Resolve transpose_neqkey_starred transpose_neqkey_Star : hprop.
+      Hint Extern 1 (Morphisms.Proper _ _) =>
+        (unfold Morphisms.Proper, Morphisms.respectful; intros; subst; 
+          repeat match goal with
+                   | [ H : heq _ _ _ _ _ _ _ |- _ ] => rewrite H
+                 end; reflexivity) : hprop.
+      Hint Extern 1 (MM.PROPS.transpose_neqkey _ _) => 
+        (clear; red; intros; subst; repeat rewrite MM.FACTS.add_o;
+          repeat match goal with 
+                   | [ |- context [ FM.E.eq_dec ?X ?Y ] ] => 
+                     destruct (FM.E.eq_dec X Y)
+                   | [ H : FM.E.eq ?X ?Y |- _ ] => rewrite H in *
+                 end; solve [ auto | exfalso; auto | heq_canceler ]) : hprop.
+
+
+      Theorem impuresD_Add : forall f argss i i',
+        MM.PROPS.Add f argss i i' ->
+        ~FM.In f i ->
+        SE.heq funcs preds U G cs
+          (impuresD i')
+          (SE.Star (starred (SE.Func f) argss SE.Emp) (impuresD i)).
+      Proof.
+        unfold impuresD; intros.
+        rewrite MM.PROPS.fold_Add; eauto with typeclass_instances hprop.
+          heq_canceler.
+      Qed.
+        
+      Theorem impuresD_Empty : forall i,
+        FM.Empty i ->
+        SE.heq funcs preds U G cs (impuresD i) SE.Emp.
+      Proof.
+        unfold impuresD; intros.
+        rewrite MM.PROPS.fold_Empty; eauto with typeclass_instances. heq_canceler.
+      Qed.
+
+      Theorem sheapD_def : forall s,
+        SE.heq funcs preds U G cs
+          (sheapD s)
+          (SE.Star (impuresD (impures s))
+                   (SE.Star (starred (@SE.Inj _ _ _) (pures s) SE.Emp)
+                            (starred (@SE.Const _ _ _) (other s) SE.Emp))).
+      Proof.
+        intros; unfold sheapD.
+        eapply MM.PROPS.fold_rec; intros.
+          rewrite impuresD_Empty; eauto. heq_canceler. 
+          rewrite impuresD_Add; eauto. heq_canceler. 
+      Qed.
+
+      Lemma sheapD_sheapD' : forall h,
+        sheapD h <===> sheapD' h.
+      Proof.
+        destruct h. rewrite sheapD_def; unfold sheapD', impuresD; simpl. 
+        repeat eapply heq_star_frame; try reflexivity.
+        generalize (@Emp types pcType stateType) at 2 3.
+        clear. intros. eapply MM.PROPS.fold_rec with (m := impures0); intros.
+          rewrite MM.PROPS.fold_Empty; eauto with typeclass_instances hprop. reflexivity.
+
+          rewrite MM.PROPS.fold_Add; eauto with typeclass_instances hprop.
+            rewrite H2. heq_canceler. 
+      Qed.
+
+      Lemma starred_In : forall T (F : T -> sexpr _ _ _) x ls' b ls,
+        (starred F (ls ++ x :: ls') b) <===> (Star (starred F (ls ++ ls') b) (F x)).
+      Proof.
+        intros. repeat rewrite starred_def. revert b.
+        induction ls; intros; simpl; heq_canceler. 
+          rewrite IHls. heq_canceler.
+      Qed.
+
+      Lemma sheapD_pures : forall stn sm h,
+        ST.satisfies cs (sexprD funcs preds U G (sheapD h)) stn sm ->
+        AllProvable funcs U G (pures h).
+      Proof.
+        intros. eapply ST.satisfies_himp in H.
+        Focus 2. rewrite sheapD_def. rewrite starred_def. reflexivity.
+        simpl in *.
+        
+        repeat match goal with
+                 | [ H : exists x, _ |- _ ] => destruct H
+                 | [ H : ST.satisfies _ (ST.star _ _) _ _ |- _ ] =>
+                   apply ST.satisfies_star in H
+                 | [ H : _ /\ _ |- _ ] => destruct H
+               end.
+        revert H2; clear. revert x1.
+        induction (pures h); simpl; auto.
+        unfold Provable. destruct (exprD funcs U G a tvProp); intros; unfold BadInj in *;
+        repeat match goal with
+                 | [ H : exists x, _ |- _ ] => destruct H
+                 | [ H : ST.satisfies _ (ST.star _ _) _ _ |- _ ] =>
+                   apply ST.satisfies_star in H
+                 | [ H : ST.satisfies _ (ST.inj _) _ _ |- _ ] =>
+                   apply ST.satisfies_pure in H
+                 | [ H : _ /\ _ |- _ ] => destruct H
+                 | [ |- _ /\ _ ] => split
+                 | [ |- _ ] => propxFo
+               end; eauto.
+      Qed.
+
+      Lemma sheapD_pull_impure : forall h f argss,
+        MM.FM.find f (impures h) = Some argss ->
+        (sheapD h) <===>
+        (Star (sheapD {| impures := MM.FM.remove f (impures h)
+          ; pures   := pures h
+          ; other   := other h |})
+        (starred (Func f) argss Emp)).
+      Proof.
+        intros. repeat rewrite sheapD_def. simpl.
+        rewrite impuresD_Add with (f := f) (argss := argss) (i := MM.FM.remove f (impures h)). 
+        heq_canceler.
+        unfold MM.PROPS.Add; intros; repeat rewrite MM.FACTS.add_o; repeat rewrite MM.FACTS.remove_o.
+        destruct (FM.E.eq_dec f y); subst; auto.
+        apply FM.remove_1; auto.
+      Qed.
+
+      Lemma fold_starred : forall X (F : nat -> X -> sexpr _ _ _) m b,
+        (MM.FM.fold (fun k ls a => Star (F k ls) a) m b) <===>
+        (Star (MM.FM.fold (fun k ls a => Star (F k ls) a) m Emp) b).
+      Proof.
+        do 2 intro.
+        intro. apply NatMap.IntMapProperties.fold_rec with (m := m).
+          intros. rewrite NatMap.IntMapProperties.fold_Empty; eauto with typeclass_instances.
+          autorewrite with hprop. reflexivity.
+
+          intros. erewrite MM.PROPS.fold_Add; eauto with typeclass_instances hprop.
+          rewrite H2. heq_canceler.
+      Qed.
+
+      Lemma starred_app : forall T (F : T -> _) a b B,
+        (starred F (a ++ b) B) <===> (starred F a (starred F b B)).
+      Proof.
+        intros; repeat rewrite starred_def.
+        induction a; simpl; intros; repeat rewrite starred_def; try reflexivity.     
+        rewrite IHa. reflexivity.
+      Qed.
+
+      Lemma multimap_join_star : forall 
+        (impures0 impures1 : MM.mmap (exprs types)) B,
+        (MM.FM.fold
+          (fun (k : nat) (ls : list (exprs types)) acc =>
+            Star (starred (Func k) ls Emp) acc)
+          (MM.mmap_join impures0 impures1) B)
+        <===>
+        (MM.FM.fold
+          (fun (k : nat) (ls : list (exprs types)) acc =>
+            Star (starred (Func k) ls Emp) acc) impures0 
+          (MM.FM.fold
+            (fun (k : nat) (ls : list (exprs types)) acc =>
+              Star (starred (Func k) ls Emp) acc) impures1 B)).
+      Proof.
+        unfold MM.mmap_join.
+        intro. apply NatMap.IntMapProperties.map_induction with (m := impures0).
+        * intros.
+          repeat rewrite NatMap.IntMapProperties.fold_Empty with (m := m); eauto with typeclass_instances.
+          reflexivity.
+
+        * intros.
+          generalize (@NatMap.IntMapProperties.fold_Add (list (exprs types)) _ (@MM.FM.Equal (list (exprs types)))).
+          intro. 
+          rewrite NatMap.IntMapProperties.fold_Equal; try solve [ clear; eauto with typeclass_instances ].
+          4: eapply H2; eauto with typeclass_instances.
+          clear H2. simpl in *.
+          unfold exprs, MM.mmap_extend; simpl in *.
+          match goal with
+            | [ |- context [ MM.FM.find ?x ?y ] ] => remember y
+          end.
+          case_eq (MM.FM.find x t); intros.
+          { subst.
+            rewrite NatMap.IntMapProperties.fold_Equal; eauto with typeclass_instances.
+            4: eapply MF.add_remove_Equal.
+            symmetry.
+            rewrite NatMap.IntMapProperties.fold_Add.
+            6: eassumption.
+            5: eauto.
+            2: eauto with typeclass_instances.
+            rewrite fold_starred.
+            rewrite NatMap.IntMapProperties.fold_Add with (m2 := impures1).
+            2: eauto with typeclass_instances.
+            instantiate (3 := x). instantiate (2 := l). 
+            instantiate (1 := MM.FM.remove x impures1). 
+            rewrite NatMap.IntMapProperties.fold_add.
+            rewrite starred_app. heq_canceler.
+          
+            generalize (@MM.mmap_join_remove_acc _ x m impures1 H0). unfold MM.mmap_join. intro.
+            symmetry. rewrite NatMap.IntMapProperties.fold_Equal.
+            5: eapply H3. clear H3.
+            rewrite H. rewrite fold_starred with (b := MM.FM.fold _ _ _). heq_canceler. eauto with typeclass_instances.
+            
+            solve [ clear; eauto with typeclass_instances hprop ].
+            solve [ clear; eauto with typeclass_instances hprop ].
+            solve [ clear; eauto with typeclass_instances hprop ].
+            solve [ clear; eauto with typeclass_instances hprop ].
+            solve [ clear; eauto with typeclass_instances hprop ].
+            apply MM.FM.remove_1; auto.
+            solve [ clear; eauto with typeclass_instances hprop ].
+            solve [ clear; eauto with typeclass_instances hprop ].
+            apply MM.FM.remove_1; auto.
+
+            { 
+              generalize MM.mmap_join_o. 
+              unfold MM.mmap_join. intros. unfold MM.mmap_extend in H3. rewrite H3 in H2; auto. 
+              apply MM.PROPS.F.not_find_in_iff in H0. unfold exprs in H0. rewrite H0 in H2.
+              
+              revert H2; clear; intros.
+              unfold NatMap.IntMapProperties.Add; intros.
+                repeat (rewrite NatMap.IntMapFacts.add_o || rewrite NatMap.IntMapFacts.remove_o).
+                destruct (NatMap.Ordered_nat.eq_dec x y); subst; auto.
+            }
+
+            solve [ clear; eauto with typeclass_instances hprop ].
+            solve [ clear; eauto with typeclass_instances hprop ].
+            solve [ clear; eauto with typeclass_instances hprop ].
+            solve [ clear; eauto with typeclass_instances hprop ].
+        }          
+        { subst.
+          rewrite NatMap.IntMapProperties.fold_add; eauto with typeclass_instances.
+          rewrite H. symmetry. rewrite fold_starred. 
+          rewrite NatMap.IntMapProperties.fold_Add; eauto with typeclass_instances.
+          symmetry. rewrite fold_starred with (b := MM.FM.fold _ _ _). heq_canceler.
+          
+          repeat (red; intros; subst). rewrite H3. heq_canceler.
+          red; intros; heq_canceler.
+          repeat (red; intros; subst). rewrite H3; heq_canceler.
+          red; intros; heq_canceler.
+          intro.
+          apply NatMap.IntMapProperties.F.in_find_iff in H3. auto.
+        }
+        eauto with typeclass_instances.
+        solve [ clear; eauto with typeclass_instances hprop ].
+        solve [ clear; eauto with typeclass_instances hprop ].
+        clear; repeat (red; intros; subst). unfold MM.mmap_extend. rewrite H.
+          destruct (MM.FM.find (elt:=list (exprs types)) y y1); try rewrite H; reflexivity.
+
+        eapply MM.transpose_neqkey_mmap_extend.
+      Qed.
+
+      Lemma star_SHeap_denote : forall s1 s2,
+        (Star (sheapD s1) (sheapD s2)) <===> (sheapD (star_SHeap s1 s2)).
+      Proof.
+        intros. symmetry. repeat rewrite sheapD_def.
+        destruct s1; destruct s2; intros; simpl; unfold star_SHeap; simpl.
+        match goal with
+          | [ |- heq _ _ _ _ _ _ (Star (Star ?FL (Star ?PL ?OL)) (Star ?FR (Star ?PR ?OR))) ] =>
+            transitivity (Star (Star FL FR) (Star (Star PL PR) (Star OL OR)))
+        end.
+        repeat rewrite starred_app.
+        unfold impuresD.
+        rewrite multimap_join_star; auto. heq_canceler.
+        rewrite <- fold_starred. heq_canceler. 
+
+        heq_canceler.
+      Qed.
+
+
+    End with_envs.
+
+    Ltac heq_canceler :=
+        repeat match goal with
+                 | [ H : SE.heq _ _ _ _ _ _ _ |- _ ] => rewrite H
+                 | [ |- context [ starred ?F ?L ?B ] ] =>
+                   match B with
+                     | SE.Emp => fail 1
+                     | _ => rewrite (@starred_base _ _ _ _ F L B)
+                   end
+               end;
+        SE_FACTS.heq_canceler.
+
+    Hint Resolve transpose_neqkey_starred transpose_neqkey_Star : hprop.
+    Hint Extern 1 (Morphisms.Proper _ _) =>
+      (unfold Morphisms.Proper, Morphisms.respectful; intros; subst; 
+        repeat match goal with
+                 | [ H : heq _ _ _ _ _ _ _ |- _ ] => rewrite H
+               end; reflexivity) : hprop.
+    Hint Extern 1 (MM.PROPS.transpose_neqkey _ _) => 
+      (clear; red; intros; subst; repeat rewrite MM.FACTS.add_o;
+        repeat match goal with 
+                 | [ |- context [ FM.E.eq_dec ?X ?Y ] ] => 
+                   destruct (FM.E.eq_dec X Y)
+                 | [ H : FM.E.eq ?X ?Y |- _ ] => rewrite H in *
+               end; solve [ auto | exfalso; auto | heq_canceler ]) : hprop.
+
+    Lemma heq_ex : forall U G cs t P Q,
+      (forall v : tvarD types t, heq funcs preds U (existT (tvarD types) t v :: G) cs P Q) ->
+      heq funcs preds U G cs (Exists t P) (Exists t Q).
+    Proof.
+      unfold heq; simpl; intros; apply ST.heq_ex; auto.
+    Qed.
+   
+    Lemma heq_existsEach : forall cs X v Y (P Q : sexpr types pcType stateType),
+      (forall Z, map (@projT1 _ _) Z = rev v -> heq funcs preds X (Z ++ Y) cs P Q) ->
+      heq funcs preds X Y cs (existsEach v P) (existsEach v Q).
+    Proof.
+      induction v; simpl; intros.
+        specialize (H nil); simpl in *; auto.
+
+        apply heq_ex. intros. eapply IHv. intros.
+        simpl. specialize (H (Z ++ @existT _ _ _ v0 :: nil)). rewrite map_app in *. 
+        rewrite H0 in *. simpl in *.
+        rewrite app_ass in *. simpl in *. auto.
+    Qed.
+
+    Lemma existsEach_app : forall X cs b a Y (P : sexpr _ _ _),
+      heq funcs preds X Y cs (existsEach a (existsEach b P)) (existsEach (a ++ b) P).
+    Proof.
+      induction a; simpl.
+      reflexivity.
+      intros. apply heq_ex; intros. apply IHa.
+    Qed.
+
+    Lemma liftSExpr_0 : forall b a, liftSExpr a 0 b = b.
+    Proof.
+      induction b; simpl; intros; auto.
+      rewrite liftExpr_0; reflexivity.
+      rewrite IHb1; rewrite IHb2; reflexivity.
+      rewrite IHb. auto.
+      f_equal. clear. induction l; simpl; auto. rewrite liftExpr_0. f_equal; auto.
+    Qed.
+    
+    Lemma sexpr_lift_ext : forall EG cs G G' s G'',
+      ST.heq cs (sexprD funcs preds EG (G'' ++ G) s) 
+      (sexprD funcs preds EG (G'' ++ G' ++ G) (liftSExpr (length G'') (length G') s)).
+    Proof.
+      induction s; simpl; intros; 
+        repeat match goal with
+                 | [ |- _ ] => rewrite <- liftExpr_ext
+                 | [ H : forall a, ST.heq _ _ _ |- _ ] => rewrite <- H
+               end; try reflexivity.
+      eapply ST.heq_ex. intros. specialize (IHs (existT (tvarD types) t v :: G'')).
+      simpl in *. auto.
+      destruct (nth_error preds f); try reflexivity.
+      clear. destruct s; simpl; clear. generalize dependent SDomain0. induction l; simpl; try reflexivity.
+      destruct SDomain0; try reflexivity.
+      rewrite <- liftExpr_ext. destruct (exprD funcs EG (G'' ++ G) a t); try reflexivity.
+      auto.
+    Qed.
+
+    Lemma star_pull_exists : forall EG cs a G s s2,
+      heq funcs preds EG G cs (Star (Exists a s) s2) (Exists a (Star s (liftSExpr 0 1 s2))).
+    Proof.
+      intros. unfold heq. simpl. rewrite ST.heq_ex_star. apply ST.heq_ex. intros.
+      apply ST.heq_star_cancel.
+      generalize (sexpr_lift_ext EG cs G (existT (tvarD types) a v :: nil) s2 nil); simpl; intro. auto.
+    Qed.            
+
+    Lemma liftSExpr_combine : forall s a b c,
+      liftSExpr a b (liftSExpr a c s) = liftSExpr a (c + b) s.
+    Proof.
+      clear. induction s; intros; simpl; 
+      repeat match goal with
+               | [ H : _ |- _ ] => rewrite H
+             end; try reflexivity. 
+      rewrite liftExpr_combine. reflexivity.
+      f_equal. rewrite map_map. apply map_ext. intros; apply liftExpr_combine.
+    Qed.
+
+    Lemma star_pull_existsEach : forall EG cs v G s s2,
+      heq funcs preds EG G cs (Star (existsEach v s) s2)
+      (existsEach v (Star s (liftSExpr 0 (length v) s2))).
+    Proof.
+      induction v; simpl.
+      intros; rewrite liftSExpr_0. reflexivity.
+
+      intros.
+      rewrite star_pull_exists. apply heq_ex. intros.
+      rewrite IHv.
+      
+      rewrite liftSExpr_combine. reflexivity.
+    Qed.
+
+
+    
+
+(*
+
+    Lemma fold_left_Star : forall T EG G cs (F : T -> _) ls base base',
+      heq EG G cs base base' ->
+      heq EG G cs (fold_left (fun acc x => Star (F x) acc) ls base)
+      (fold_left (fun acc x => Star (F x) acc) ls base').
+    Proof.
+      induction ls; simpl; intros; auto.
+      rewrite IHls. reflexivity. apply heq_star_frame; auto; reflexivity.
+    Qed.
+*)
+
+    Lemma starred_liftSExpr : forall F a b (ls : list (expr types)) base,
+      (forall a0, liftSExpr a b (F a0) = F (liftExpr a b a0)) ->
+      liftSExpr a b (starred F ls base) = starred F (map (liftExpr a b) ls) (liftSExpr a b base).
+    Proof.
+      induction ls; simpl; intros; try reflexivity.
+      case_eq (starred F ls base); intros;
+        rewrite <- IHls; repeat rewrite H0; simpl; repeat rewrite H; simpl; eauto.
+    Qed.
+
+    Lemma liftSExpr_existsEach : forall EG cs v0 s G n v,
+      heq funcs preds EG G cs (liftSExpr n v (existsEach v0 s)) 
+                  (existsEach v0 (liftSExpr (n + length v0) v s)).
+    Proof.
+      induction v0; simpl; intros.
+        intros. rewrite Plus.plus_0_r. reflexivity.
+      
+        apply heq_ex; intros. rewrite IHv0. cutrewrite (S n + length v0 = n + S (length v0)); try reflexivity; omega.
+    Qed.
+
+    Lemma skipn_skipn : forall T a (ls : list T) b,
+      skipn b (skipn a ls) = skipn (b + a) ls.
+    Proof.
+      clear; induction a; simpl; intros.
+        rewrite Plus.plus_0_r. auto.
+        rewrite Plus.plus_comm. simpl. destruct ls; auto. destruct b; auto.
+        rewrite IHa. rewrite Plus.plus_comm. auto.
+    Qed.
+
+    Lemma heq_liftSExpr : forall cs EG G G' G'' P Q,
+      heq funcs preds EG (G ++ G'') cs P Q ->
+      heq funcs preds EG (G ++ G' ++ G'') cs (liftSExpr (length G) (length G') P) (liftSExpr (length G) (length G') Q).
+    Proof.
+      unfold heq; intros.
+      repeat rewrite <- sexpr_lift_ext. auto.
+    Qed.
+
+
+
+    Lemma sheapD_sexprD_liftVars : forall EG cs s G G' G'',
+      heq funcs preds EG (G ++ G' ++ G'') cs
+        (liftSExpr (length G) (length G') (sheapD' s))
+        (sheapD' (sheap_liftVars (length G) (length G') s)).
+    Proof.
+      destruct s; unfold sheap_liftVars, sheapD'; simpl; intros; repeat apply heq_star_frame; intros.
+
+      clear. change Emp with (liftSExpr (length G) (length G') Emp) at 2. generalize (@Emp types pcType stateType).
+        unfold MM.mmap_map. intros. rewrite MF.fold_map_fusion; eauto with typeclass_instances.
+
+        Focus. 
+        revert s.
+        apply NatMap.IntMapProperties.map_induction with (m := impures0); intros.
+        repeat (rewrite MM.PROPS.fold_Empty; eauto with typeclass_instances). reflexivity.
+
+        symmetry. rewrite MM.PROPS.fold_Add. 6: eauto. 5: eauto. 2: eauto with typeclass_instances.
+        rewrite starred_base. rewrite <- H. clear H.
+        assert (forall base, heq funcs preds EG (G ++ G' ++ G'') cs 
+          (starred (Func x) (map (map (liftExpr (length G) (length G'))) e) (liftSExpr (length G) (length G') base))
+          (liftSExpr (length G) (length G') (starred (Func x) e base))).
+        { clear.
+          induction e; intros; try reflexivity. rewrite starred_def. simpl. rewrite <- starred_def.
+            rewrite IHe. solve [ destruct (starred (Func x) e base); simpl; heq_canceler ]. 
+        }
+        rewrite H with (base := Emp).
+        change (Star 
+        (liftSExpr (length G) (length G')
+           (MM.FM.fold
+              (fun (k : MM.FM.key) => starred (Func k)) m s))
+(liftSExpr (length G) (length G') (starred (Func x) e Emp)))
+        with (liftSExpr (length G) (length G')
+          (Star 
+            (MM.FM.fold
+              (fun (k : MM.FM.key) => starred (Func k)) m s)
+(starred (Func x) e Emp))).
+
+        eapply heq_liftSExpr.
+                
+        symmetry.
+        rewrite MM.PROPS.fold_Add. 6: eauto. rewrite <- starred_base. reflexivity.
+        eauto with typeclass_instances hprop.
+        eauto with typeclass_instances hprop.
+        clear; red; intros; subst; repeat rewrite MM.FACTS.add_o;
+          repeat match goal with 
+                   | [ |- context [ FM.E.eq_dec ?X ?Y ] ] => 
+                     destruct (FM.E.eq_dec X Y)
+                   | [ H : FM.E.eq ?X ?Y |- _ ] => rewrite H in *
+                 end; auto.
+        heq_canceler.
+        eauto with typeclass_instances hprop.
+        clear; do 4 (red; intros; subst); heq_canceler.
+
+        clear; red; intros; subst; repeat rewrite MM.FACTS.add_o.
+        heq_canceler.
+        eapply transpose_neqkey_starred.
+        
+        Opaque starred.
+        symmetry. rewrite starred_def. induction pures0; try reflexivity.
+        simpl. rewrite IHpures0.
+        match goal with
+          | [ |- heq _ _ _ _ _ ?X _ ] =>
+            change X with
+              (liftSExpr (length G) (length G') (Star (Inj a) (starred (@Inj types pcType stateType) pures0 Emp)))
+        end.
+        apply heq_liftSExpr. symmetry. repeat rewrite starred_def. simpl. heq_canceler.
+
+        symmetry. etransitivity. rewrite starred_def. reflexivity. induction other0; try reflexivity.
+        simpl. rewrite IHother0.
+        match goal with
+          | [ |- heq _ _ _ _ _ ?X _ ] =>
+            change X with
+              (liftSExpr (length G) (length G') (Star (Const a) (starred (@Const types pcType stateType) other0 Emp)))
+        end.
+        apply heq_liftSExpr. symmetry. repeat rewrite starred_def. simpl. reflexivity.
+    Qed.
+
+    Lemma hash_denote' : forall EG cs (s : sexpr _ _ _) G, 
+      heq funcs preds EG G cs s (existsEach (fst (hash s)) (sheapD' (snd (hash s)))).
+    Proof.
+      Opaque star_SHeap.
+      induction s; simpl; try solve [ unfold sheapD'; simpl; intros; repeat (rewrite heq_star_emp_r || rewrite heq_star_emp_l); reflexivity ].
+        (** Exists **)
+        Focus 2.
+        unfold sheapD'; simpl; intros. case_eq (hash s); intros; simpl.
+        eapply heq_ex. intros. specialize (IHs (existT (tvarD types) t v0 :: G)). simpl in *.
+        rewrite H in IHs. simpl in *. eauto.
+
+        (** Star **)
+        Focus.
+        intros. rewrite IHs1 at 1. intros.
+        destruct (hash s1); destruct (hash s2); simpl in *.
+        rewrite IHs2.
+        rewrite <- (@existsEach_app EG cs) with (Y := G).
+        rewrite star_pull_existsEach. apply heq_existsEach. intros.
+        rewrite heq_star_comm.
+
+        rewrite liftSExpr_existsEach.
+        rewrite star_pull_existsEach. eapply heq_existsEach; intros.
+        generalize star_SHeap_denote.
+        symmetry. rewrite <- sheapD_sheapD'.
+        rewrite <- star_SHeap_denote. simpl plus.
+        cutrewrite (length v0 = length Z0).
+        cutrewrite (length v = length Z).
+        repeat rewrite sheapD_sheapD'.
+        rewrite sheapD_sexprD_liftVars.
+        rewrite sheapD_sexprD_liftVars with (G := nil). heq_canceler.
+        rewrite <- rev_length; rewrite <- H; apply map_length.
+        rewrite <- rev_length; rewrite <- H0; apply map_length.
+    Qed.
+    
+    Theorem hash_denote : forall EG G cs (s : sexpr _ _ _), 
+      heq funcs preds EG G cs s (existsEach (fst (hash s)) (sheapD (snd (hash s)))).
+    Proof.
+      intros. specialize (@hash_denote' EG cs s G). etransitivity.
+      eassumption. apply heq_existsEach. intros. rewrite sheapD_sheapD'. reflexivity.
+    Qed.
+
+    (** replace "real" variables [a,b) and replace them with
+     ** uvars [c,..]
+     **)
+    Definition sheapSubstU (a b c : nat) (s : SHeap) : SHeap :=
+      {| impures := MM.mmap_map (map (exprSubstU a b c)) (impures s)
+       ; pures := map (exprSubstU a b c) (pures s)
+       ; other := other s
+       |}.
+
+  End env.
+
+  Implicit Arguments Emp [ types pcType stateType ].
+  Implicit Arguments Star [ types pcType stateType ].
+  Implicit Arguments Exists [ types pcType stateType ].
+  Implicit Arguments Func [ types pcType stateType ].
+  Implicit Arguments Const [ types pcType stateType ].
+  Implicit Arguments Inj [ types pcType stateType ].
+
+
+  Lemma change_ST_himp_himp : forall (types : list type)
+    (funcs : functions types) (pc st : tvar)
+    (sfuncs : list (ssignature types pc st))
+    EG G
+    (cs : codeSpec (tvarD types pc) (tvarD types st))
+    (L R : sexpr types pc st),
+    himp funcs sfuncs EG G cs L R ->
+    ST.himp cs
+      (@sexprD types pc st funcs sfuncs EG G L)
+      (@sexprD types pc st funcs sfuncs EG G R).
+  Proof.
+    unfold himp. intros. auto.
+  Qed.
+
+End Make.
